LeanMqtt.lean
@@ -1,3 +1,4 @@
 -- This module serves as the root of the `LeanMqtt` library.
 -- Import modules here that should be built as part of the library.
-import LeanMqtt.Basic
+import LeanMqtt.Defs.Packets.Packet
+import LeanMqtt.Serialization.Packets.Packet
