LeanMqtt/Core/Parser.lean
@@ -1,0 +1,5 @@
+abbrev Parser (α : Type) := StateT (List UInt8) Option α
+
+theorem parser_app_is_run {α} {l : List UInt8} (p : Parser α) :
+  p l = p.run l :=
+  rfl
