LeanMqtt/Defs/Packets/FixedHeader.lean
@@ -1,0 +1,53 @@
+import LeanMqtt.Defs.Primitives
+
+namespace Mqtt
+
+inductive WhichPkt where
+  | connect
+  | connack
+  | publish
+  | puback
+  | pubrec
+  | pubrel
+  | pubcomp
+  | subscribe
+  | suback
+  | unsubscribe
+  | unsuback
+  | pingreq
+  | pingresp
+  | disconnect
+  | auth
+deriving Repr, BEq
+
+instance : Inhabited WhichPkt where
+  default := .pingreq
+
+structure PublishFlags where
+  dup : BitVec 1
+  qos : BitVec 2
+  retain : BitVec 1
+
+def WhichPkt.flagType : WhichPkt → Type
+  | .connect     => { i : BitVec 4 // i = 0b0000 }
+  | .connack     => { i : BitVec 4 // i = 0b0000 }
+  | .publish     => PublishFlags
+  | .puback      => { i : BitVec 4 // i = 0b0000 }
+  | .pubrec      => { i : BitVec 4 // i = 0b0000 }
+  | .pubrel      => { i : BitVec 4 // i = 0b0010 }
+  | .pubcomp     => { i : BitVec 4 // i = 0b0000 }
+  | .subscribe   => { i : BitVec 4 // i = 0b0010 }
+  | .suback      => { i : BitVec 4 // i = 0b0000 }
+  | .unsubscribe => { i : BitVec 4 // i = 0b0010 }
+  | .unsuback    => { i : BitVec 4 // i = 0b0000 }
+  | .pingreq     => { i : BitVec 4 // i = 0b0000 }
+  | .pingresp    => { i : BitVec 4 // i = 0b0000 }
+  | .disconnect  => { i : BitVec 4 // i = 0b0000 }
+  | .auth        => { i : BitVec 4 // i = 0b0000 }
+
+structure FixedHeader where
+  which : WhichPkt
+  flags : WhichPkt.flagType which
+  size  : VarInt -- TODO: depend on information after
+
+end Mqtt
