LeanMqtt/Defs/Packets/Packet.lean
@@ -1,0 +1,16 @@
+import LeanMqtt.Defs.Packets.FixedHeader
+import LeanMqtt.Defs.Packets.VarHeader
+import LeanMqtt.Defs.Packets.Payload
+
+namespace Mqtt
+
+structure Header where
+  fix : FixedHeader
+  var : VarHeader fix
+
+structure Packet where
+  fixed_header : FixedHeader
+  var_header   : VarHeader fixed_header
+  payload      : Payload
+
+end Mqtt
