LeanMqtt/Defs/Packets/Properties.lean
@@ -1,0 +1,11 @@
+import LeanMqtt.Core.WithLength
+import LeanMqtt.Serialization.Packets.Property
+
+namespace Mqtt
+
+instance : GetLength (List Property) where
+  length l := l.foldl (fun acc p => acc + (Property.serialize p).length) 0 -- Placeholder, will be fixed
+
+abbrev Properties := WithLength (List Property) VarInt
+
+end Mqtt
