LeanMqtt/Packets/Proofs.lean
@@ -1,9 +1,0 @@
-import LeanMqtt.Packets.Packet
-import LeanMqtt.Primitives
-import LeanMqtt.Serialization
-import LeanMqtt.WithLength
-import LeanMqtt.Packets.Packet.FixedHeader
-
-namespace Mqtt
-
-end Mqtt
