LeanMqtt/Proofs/Packets/FixedHeader.lean
@@ -1,0 +1,51 @@
+import LeanMqtt.Serialization.Packets.FixedHeader
+import LeanMqtt.Proofs.Primitives
+import Std.Tactic.BVDecide
+
+namespace Mqtt
+open Mqtt
+
+theorem WhichPkt.encode_decode (which : WhichPkt) :
+  WhichPkt.decode? which.encode = which := by
+  cases which <;> rfl
+
+theorem WhichPkt.encode_decode_flags (which : WhichPkt) (flags : WhichPkt.flagType which) :
+  WhichPkt.decodeFlags which (WhichPkt.encodeFlags which flags) = some flags := by
+  cases which <;> simp [WhichPkt.encodeFlags, WhichPkt.decodeFlags]
+  case publish =>
+    have h₁ : BitVec.extractLsb 3 3 (flags.dup ++ flags.qos ++ flags.retain) = flags.dup := by bv_decide
+    have h₂ : BitVec.extractLsb 2 1 (flags.dup ++ flags.qos ++ flags.retain) = flags.qos := by bv_decide
+    have h₃ : BitVec.extractLsb 0 0 (flags.dup ++ flags.qos ++ flags.retain) = flags.retain := by bv_decide
+    rw [h₁, h₂, h₃]
+    rfl
+  all_goals {
+    have : flags.val = _ := flags.property
+    simp only [this, BitVec.ofNat_eq_ofNat, exists_true_left]
+    exact Subtype.ext flags.property.symm
+  }
+
+theorem WhichPkt.roundtrip (which : WhichPkt) (flags : WhichPkt.flagType which) (rest : List UInt8) :
+  WhichPkt.parser.run (WhichPkt.serialize which flags ++ rest) = some (⟨which, flags⟩, rest) := by
+  simp only [WhichPkt.parser, WhichPkt.serialize,]
+  simp only [
+    bind_pure_comp, BitVec.append_eq, Nat.reduceAdd, StateT.run_bind,
+    StateT.run_monadLift, monadLift_self, Option.pure_def, Option.bind_eq_bind,
+    Option.bind, StateT.run_map, Option.map_eq_map
+  ]
+  simp only [UInt8.roundtrip _ _]
+  have : BitVec.extractLsb 7 4 (which.encode ++ which.encodeFlags flags) = which.encode :=
+    by bv_decide
+  rw [this]
+  simp [WhichPkt.encode_decode]
+  have : BitVec.extractLsb 3 0 (which.encode ++ which.encodeFlags flags) = which.encodeFlags flags :=
+    by bv_decide
+  rw [this]
+  simp [WhichPkt.encode_decode_flags]
+
+theorem FixedHeader.roundtrip (header : FixedHeader) (rest : List UInt8) :
+  FixedHeader.parser.run (header.serialize ++ rest) = some (header, rest) := by
+  simp [FixedHeader.parser, FixedHeader.serialize]
+  simp [WhichPkt.roundtrip header.which header.flags]
+  simp [VarInt.roundtrip _]
+
+end Mqtt
