LeanMqtt/Proofs/Packets/Packet.lean
@@ -1,0 +1,13 @@
+import LeanMqtt.Serialization.Packets.Packet
+import LeanMqtt.Proofs.Packets.FixedHeader
+import LeanMqtt.Proofs.Packets.VarHeader
+
+namespace Mqtt
+
+def Header.roundtrip (h : Header) (rest : List UInt8) :
+  parser.run (h.serialize ++ rest) = some (h, rest) := by
+  simp [parser, serialize]
+  simp [FixedHeader.roundtrip]
+  simp [VarHeader.roundtrip]
+
+end Mqtt
