LeanMqtt/Proofs/Packets/Properties.lean
@@ -1,0 +1,17 @@
+import LeanMqtt.Serialization.Packets.Properties
+import LeanMqtt.Proofs.Primitives
+import LeanMqtt.Proofs.Packets.Property
+
+namespace Mqtt
+
+-- TODO: prove
+theorem parsePropsLoop_len (chunk : List UInt8) (l : List Property) :
+  parsePropsLoop chunk = some l → chunk.length = (l.foldl (fun acc p => acc + p.byteSize) 0) := by
+  -- simp [GetLength.length]
+  sorry
+
+theorem Properties.roundtrip (ps : Properties) (rest : List UInt8) :
+  Properties.parser.run (ps.serialize ++ rest) = some (ps, rest) := by
+  sorry
+
+end Mqtt
