LeanMqtt/Proofs/Packets/Property.lean
@@ -1,0 +1,27 @@
+import LeanMqtt.Serialization.Packets.Property
+import LeanMqtt.Proofs.Primitives
+
+namespace Mqtt
+
+def Property.roundtrip_kind (k : Property.Kind) (val : Property.typeOfKind k) (rest : List UInt8) :
+  (Property.parserKind k).run (Property.serializeKind k val ++ rest) = some (val, rest) := by
+  simp [Property.parserKind, Property.serializeKind]
+  split
+  repeat' simp only
+  · simp only [UInt8.roundtrip]
+  · simp only [UInt16.roundtrip]
+  · simp only [UInt32.roundtrip]
+  · simp only [VarInt.roundtrip]
+  · simp only [BinaryData.roundtrip]
+  · simp only [Str.roundtrip]
+  · simp only [StrPair.roundtrip]
+  · contradiction
+
+theorem Property.roundtrip (p : Property) (rest : List UInt8) :
+  Property.parser.run (p.serialize ++ rest) = some (p, rest) := by
+  simp [Property.parser, Property.serialize]
+  simp [Option.bind, Option.map]
+  simp [VarInt.roundtrip]
+  simp [Property.roundtrip_kind]
+
+end Mqtt
