LeanMqtt/Proofs/Packets/VarHeader.lean
@@ -1,0 +1,124 @@
+import LeanMqtt.Serialization.Packets.VarHeader
+import LeanMqtt.Proofs.Packets.Properties
+import LeanMqtt.Proofs.Primitives
+
+namespace Mqtt
+
+def Var_Connect.roundtrip (v : Var_Connect) (rest : List UInt8) :
+  Var_Connect.parser.run (v.serialize ++ rest) = some (v, rest) := by
+  simp [Var_Connect.parser, Var_Connect.serialize]
+  simp [Str.roundtrip]
+  simp [UInt8.roundtrip]
+  simp [Properties.roundtrip]
+
+theorem Var_Connack.roundtrip (v : Var_Connack) (rest : List UInt8) :
+  Var_Connack.parser.run (v.serialize ++ rest) = some (v, rest) := by
+  simp [Var_Connack.parser, Var_Connack.serialize]
+  simp [UInt8.roundtrip, Properties.roundtrip]
+
+theorem Var_Publish.roundtrip {qos} (v : Var_Publish qos) (rest : List UInt8) :
+  (Var_Publish.parser qos).run (v.serialize ++ rest) = some (v, rest) := by
+  simp [Var_Publish.parser, Var_Publish.serialize]
+  simp [Str.roundtrip]
+
+  split
+  · next h_qos =>
+    -- Case: QoS > 0
+    simp [UInt16.roundtrip]
+    simp [Properties.roundtrip]
+  · next h_qos =>
+    -- Case: QoS == 0
+    simp [Properties.roundtrip]
+    congr
+    have h_zero : qos = 0 := by bv_decide
+    subst h_zero
+    simp
+    apply Subsingleton.elim () v.packet_id
+
+theorem Var_Puback.roundtrip (v : Var_Puback) (rest : List UInt8) :
+  parser.run (v.serialize ++ rest) = some (v, rest) := by
+  simp [Var_Puback.parser, Var_Puback.serialize]
+  simp [UInt16.roundtrip, UInt8.roundtrip, Properties.roundtrip]
+
+theorem Var_Pubrec.roundtrip (v : Var_Pubrec) (rest : List UInt8) :
+  parser.run (v.serialize ++ rest) = some (v, rest) := by
+  simp [parser, serialize]
+  simp [UInt16.roundtrip, UInt8.roundtrip, Properties.roundtrip]
+
+theorem Var_Pubrel.roundtrip (v : Var_Pubrel) (rest : List UInt8) :
+  parser.run (v.serialize ++ rest) = some (v, rest) := by
+  simp [parser, serialize]
+  simp [UInt16.roundtrip, UInt8.roundtrip, Properties.roundtrip]
+
+theorem Var_Pubcomp.roundtrip (v : Var_Pubcomp) (rest : List UInt8) :
+  parser.run (v.serialize ++ rest) = some (v, rest) := by
+  simp [parser, serialize]
+  simp [UInt16.roundtrip, UInt8.roundtrip, Properties.roundtrip]
+
+theorem Var_Subscribe.roundtrip (v : Var_Subscribe) (rest : List UInt8) :
+  parser.run (v.serialize ++ rest) = some (v, rest) := by
+  simp [parser, serialize]
+  simp [UInt16.roundtrip, Properties.roundtrip]
+
+theorem Var_Suback.roundtrip (v : Var_Suback) (rest : List UInt8) :
+  parser.run (v.serialize ++ rest) = some (v, rest) := by
+  simp [parser, serialize]
+  simp [UInt16.roundtrip, Properties.roundtrip]
+
+theorem Var_Unsubscribe.roundtrip (v : Var_Unsubscribe) (rest : List UInt8) :
+  parser.run (v.serialize ++ rest) = some (v, rest) := by
+  simp [parser, serialize]
+  simp [UInt16.roundtrip, Properties.roundtrip]
+
+theorem Var_Unsuback.roundtrip (v : Var_Unsuback) (rest : List UInt8) :
+  parser.run (v.serialize ++ rest) = some (v, rest) := by
+  simp [parser, serialize]
+  simp [UInt16.roundtrip, Properties.roundtrip]
+
+theorem Var_Pingreq.roundtrip (v : Var_Pingreq) (rest : List UInt8) :
+  parser.run (v.serialize ++ rest) = some (v, rest) := by
+  simp [parser, serialize]
+
+theorem Var_Pingresp.roundtrip (v : Var_Pingresp) (rest : List UInt8) :
+  parser.run (v.serialize ++ rest) = some (v, rest) := by
+  simp [parser, serialize]
+
+theorem Var_Disconnect.roundtrip (v : Var_Disconnect) (rest : List UInt8) :
+  parser.run (v.serialize ++ rest) = some (v, rest) := by
+  simp [parser, serialize]
+  simp [UInt8.roundtrip, Properties.roundtrip]
+
+theorem Var_Auth.roundtrip (v : Var_Auth) (rest : List UInt8) :
+  parser.run (v.serialize ++ rest) = some (v, rest) := by
+  simp [parser, serialize]
+  simp [UInt8.roundtrip, Properties.roundtrip]
+
+theorem VarHeader.roundtrip_value
+  {w : WhichPkt} {f : WhichPkt.flagType w} (v : VarHeader.getType w f) (rest : List UInt8) :
+  (VarHeader.parserValue w f).run (VarHeader.serializeValue v ++ rest) = some (v, rest) := by
+  simp [parserValue, serializeValue]
+  split
+  repeat' simp only
+  · simp [Var_Connect.roundtrip _ _]
+  · simp [Var_Connack.roundtrip _ _]
+  · simp [Var_Publish.roundtrip _ _]
+  · simp [Var_Puback.roundtrip _ _]
+  · simp [Var_Pubrec.roundtrip _ _]
+  · simp [Var_Pubrel.roundtrip _ _]
+  · simp [Var_Pubcomp.roundtrip _ _]
+  · simp [Var_Subscribe.roundtrip _ _]
+  · simp [Var_Suback.roundtrip _ _]
+  · simp [Var_Unsubscribe.roundtrip _ _]
+  · simp [Var_Unsuback.roundtrip _ _]
+  · simp [Var_Pingreq.roundtrip _ _]
+  · simp [Var_Pingresp.roundtrip _ _]
+  · simp [Var_Disconnect.roundtrip _ _]
+  · simp [Var_Auth.roundtrip _ _]
+
+
+theorem VarHeader.roundtrip (h : FixedHeader) (v : VarHeader h) (rest : List UInt8) :
+  (parser h).run (v.serialize h ++ rest) = some (v, rest) := by
+  simp [parser, serialize]
+  simp [VarHeader.roundtrip_value v]
+
+end Mqtt
