LeanMqtt/Serialization/Packets/FixedHeader.lean
@@ -1,0 +1,111 @@
+import LeanMqtt.Core.Parser
+import LeanMqtt.Defs.Packets.FixedHeader
+import LeanMqtt.Serialization.Primitives
+
+private instance (r : Std.Range) (i : Nat) : Decidable (i ∈ r) := by
+  dsimp [Membership.mem]
+  infer_instance
+
+namespace Mqtt
+open Mqtt
+
+def WhichPkt.encode (pkt : WhichPkt) : BitVec 4 :=
+  match pkt with
+  | .connect     => 1
+  | .connack     => 2
+  | .publish     => 3
+  | .puback      => 4
+  | .pubrec      => 5
+  | .pubrel      => 6
+  | .pubcomp     => 7
+  | .subscribe   => 8
+  | .suback      => 9
+  | .unsubscribe => 10
+  | .unsuback    => 11
+  | .pingreq     => 12
+  | .pingresp    => 13
+  | .disconnect  => 14
+  | .auth        => 15
+
+def WhichPkt.decode? : BitVec 4 → Option WhichPkt
+  | 1 => some .connect
+  | 2 => some .connack
+  | 3 => some .publish
+  | 4 => some .puback
+  | 5 => some .pubrec
+  | 6 => some .pubrel
+  | 7 => some .pubcomp
+  | 8 => some .subscribe
+  | 9 => some .suback
+  | 10 => some .unsubscribe
+  | 11 => some .unsuback
+  | 12 => some .pingreq
+  | 13 => some .pingresp
+  | 14 => some .disconnect
+  | 15 => some .auth
+  | _ => none
+
+def WhichPkt.encodeFlags (which : WhichPkt) (flags : WhichPkt.flagType which) : BitVec 4 :=
+  match which with
+  | .publish =>
+    flags.dup
+    |>.append flags.qos
+    |>.append flags.retain
+    | .connect     => flags.val
+    | .connack     => flags.val
+    | .puback      => flags.val
+    | .pubrec      => flags.val
+    | .pubrel      => flags.val
+    | .pubcomp     => flags.val
+    | .subscribe   => flags.val
+    | .suback      => flags.val
+    | .unsubscribe => flags.val
+    | .unsuback    => flags.val
+    | .pingreq     => flags.val
+    | .pingresp    => flags.val
+    | .disconnect  => flags.val
+    | .auth        => flags.val
+
+def WhichPkt.decodeFlags (which : WhichPkt) (flagsBv4 : BitVec 4) : Option (WhichPkt.flagType which) :=
+  match which with
+  | .publish =>
+    let dup    := flagsBv4.extractLsb 3 3
+    let qos    := flagsBv4.extractLsb 2 1
+    let retain := flagsBv4.extractLsb 0 0
+    some { dup, qos, retain }
+  -- Flags must be 0b10
+  | .pubrel | .subscribe | .unsubscribe =>
+    if h : flagsBv4 = 0b0010 then some ⟨flagsBv4, h⟩ else none
+  -- Flags must be 0b00
+  | .connect  | .connack | .puback   | .pubrec     | .pubcomp | .suback
+  | .unsuback | .pingreq | .pingresp | .disconnect | .auth =>
+    if h : flagsBv4 = 0b0000 then some ⟨flagsBv4, h⟩ else none
+
+def WhichPkt.serialize (which : WhichPkt) (flags : WhichPkt.flagType which) : List UInt8 :=
+  let byte := which
+    |>.encode
+    |>.append (which.encodeFlags flags)
+  UInt8.ofBitVec byte |>.serialize
+
+def WhichPkt.parser : Parser ((which : WhichPkt) × WhichPkt.flagType which) := do
+  let byte ← UInt8.parser
+  let bv := byte.toBitVec
+
+  let whichBits := bv.extractLsb 7 4
+  let flagsBits := bv.extractLsb 3 0
+
+  let which ← WhichPkt.decode? whichBits
+  let flags ← WhichPkt.decodeFlags which flagsBits
+  return ⟨which, flags⟩
+
+def FixedHeader.serialize : FixedHeader → List UInt8 :=
+  fun ⟨which, flags, size⟩ =>
+    let byte1 := which.serialize flags
+    byte1 ++ (VarInt.serialize size)
+
+def FixedHeader.parser : Parser FixedHeader := do
+  let ⟨which, flags⟩ ← WhichPkt.parser
+  let size ← VarInt.parser
+  return { which, flags, size }
+
+end Mqtt
